*Executed from: BF00757025/section3.py*
## Equations (18) and (19)
Let us suppose $P = $ $\left[\begin{matrix}- \frac{1}{{}^1u_1} & \frac{1}{{}^1u_2}\\- \frac{{}^2u_1}{{}^1u_1} & \frac{{}^2u_2}{{}^1u_2}\end{matrix}\right]$
## Equations (21) and (22)
$g^{11} = {}_2 u^{1} = $ $- \frac{{}^1u_2}{{}^1u_1 {}^2u_2 - {}^1u_2 {}^2u_1}$
$- \frac{{}^1u_2}{{}^1u_1 {}^2u_2 - {}^1u_2 {}^2u_1}$
A == B is True
$g^{22} = {}_2 u^{2} = $ $\frac{{}^1u_1}{{}^1u_1 {}^2u_2 - {}^1u_2 {}^2u_1}$
$\frac{{}^1u_1}{{}^1u_1 {}^2u_2 - {}^1u_2 {}^2u_1}$
A == B is True
## Equations (23) and (24)
$K^{11} = {}_a u^{b} = $ $\frac{{}^2u_2}{{}^1u_1 {}^2u_2 - {}^1u_2 {}^2u_1}$
$\frac{{}^2u_2}{{}^1u_1 {}^2u_2 - {}^1u_2 {}^2u_1}$
A == B is True
$K^{22} = {}_a u^{b} = $ $- \frac{{}^2u_1}{{}^1u_1 {}^2u_2 - {}^1u_2 {}^2u_1}$
$- \frac{{}^2u_1}{{}^1u_1 {}^2u_2 - {}^1u_2 {}^2u_1}$
A == B is True
